---
title: "The Binomial No-Arbitrage Pricing Model"
description: |
  This is a proposition of solutions to the exercises in the chapter 1 of the book "Stochastic Calculus for Finance I: The Binomial Asset Pricing Model" by Steven Shreve.
author:
  - name: QuantBender 
    url: https://quantbender.github.io
    affiliation: UM6P
    affiliation_url: http://www.um6p.ma/
date: "`r Sys.Date()`"
output: distill::distill_article
---

```{r setup, include=FALSE}
knitr::opts_chunk$set(echo = FALSE)
```

## Exercise 1.1

Assume in one-period binomial market of Section 1.1 that both H and T have positive probability of occuring. Show that condition (1.1.2) precludes arbitrage. In other words, show that if $X_0=0$ and $X_1=\Delta_0 S_1 + (1+r)(X_0-\Delta_0 S_0)$ then we cannot have $X_1$ strictly positive with positive probability unless $X_1$ is strictly negative with positive probability as well, and this is the case regardless of the choice of the number $\Delta_0$.

**Answer:**

The condition (1.1.2) is given by:

**In the one-period binomial model, to rule out arbitrage we must assume $0 < d < 1+r < u$.**

Arbitrage is a trading strategy that involves no initial investment and has a positive probability of making a profit. 

Let's assume that $X_0=0$ and $X_1=\Delta_0 S_1 + (1+r)(X_0-\Delta_0 S_0)$ for two possible states of the world $H$ and $T$. We have:

$$
\begin{aligned}
\begin{cases}
X_1(H) &= \Delta_0 S_1(H) + (1+r)(X_0-\Delta_0 S_0(H)) \\
X_1(T) &= \Delta_0 S_1(T) + (1+r)(X_0-\Delta_0 S_0(T))
\end{cases}\\
&\Rightarrow
\begin{cases}
X_1(H) &= \Delta_0 u S_0 + (1+r)(X_0-\Delta_0 S_0) \\
X_1(T) &= \Delta_0 d S_0 + (1+r)(X_0-\Delta_0 S_0)
\end{cases}\\
&\Rightarrow
\begin{cases}
\Delta_{0} = \frac{X_1(H) - (1+r)X_0}{uS_0 - (1+r)S_0} \\
X_1(T) = \frac{X_1(H) - (1+r)X_0}{uS_0 - (1+r)S_0} d S_0 + (1+r)(X_0-\frac{X_1(H) - (1+r)X_0}{uS_0 - (1+r)S_0} S_0)
\end{cases}\\
&\Rightarrow 
X_1(T) = \frac{X_1(H) - (1+r)X_0}{u - (1+r)} d + (1+r)(X_0-\frac{X_1(H) - (1+r)X_0}{u - (1+r)})\\
&\Rightarrow
X_1(T)(u-1-r) = dX_1(H) - (1+r)dX_0 - X_1(H) + (1+r)(u-1-r)X_0 - (1+r)X_1(H) + (1+r)^2 X_0\\
&\Rightarrow
X_1(T)(u-1-r) = (d - 1 - r)X_1(H) + (1+r)(-d+u-1-r+1+r)X_0\\
&\Rightarrow
X_1(T)(u-1-r) = (d - 1 - r)X_1(H) + (1+r)(u-d)X_0\\
&\Rightarrow
0 = X_0 = \frac{1}{1+r}[\frac{u-1-r}{u-d}X_1(T)+\frac{1+r-d}{u-d}X_1(H)]\\
&\Rightarrow
0 = X_0 = (u-1-r)X_1(T)+(1+r-d)X_1(H)]\\
\end{aligned}
$$
From condition 1.1.2, we have $0 < d < 1+r < u$. This implies that $u-1-r > 0$ and $1+r-d > 0$. Therefore, if $X_1(T) > 0$ then $X_1(H) < 0$ and vice versa. This shows that if $X_1$ is strictly positive with positive probability, then $X_1$ is strictly negative with positive probability as well.

Hence the condition (1.1.2) precludes arbitrage.

## Exercise 1.2
